Use implicit types to avoid program definitions in LR

theories/iris/logrel/relations.v
@@ -21,8 +21,6 @@ Section Relations.
 
   Variable sr : store_runtime.
 
-  Obligation Tactic := try solve_proper.
-
   Definition ns_func (x : N) : namespace := nroot .@ "rwf" .@ x.
 
   Notation VR := (leibnizO val -n> iPropO Σ).
@@ -33,15 +31,20 @@ Section Relations.
   Notation ClR := (leibnizO function_closure -n> iPropO Σ).
   Notation ER := (leibnizO (lholed * list administrative_instruction) -n> iPropO Σ).
 
-  Implicit Types L : leibnizO R.Local_Ctx.
-  Implicit Types WL : leibnizO wlocal_ctx.
+  Implicit Type L : leibnizO R.Local_Ctx.
+  Implicit Type WL : leibnizO wlocal_ctx.
 
-  Implicit Types v : leibnizO val.
-  Implicit Types f : leibnizO frame.
-  Implicit Types cl : leibnizO function_closure.
-  Implicit Types i : leibnizO instance.
+  Implicit Type v : leibnizO val.
+  Implicit Type ws : leibnizO (list value).
+  Implicit Type bs : leibnizO bytes.
+  Implicit Type f : leibnizO frame.
+  Implicit Type cl : leibnizO function_closure.
+  Implicit Type lh_es : leibnizO (lholed * list administrative_instruction).
+  Implicit Type i : leibnizO instance.
 
-  Implicit Types τf : leibnizO R.FunType.
+  Implicit Type τ : leibnizO R.Typ.
+  Implicit Type τs : leibnizO (list R.Typ).
+  Implicit Type τf : leibnizO R.FunType.
 
   Definition relations : Type :=
     (* Physical Value *)
@@ -49,80 +52,55 @@ Section Relations.
     (* Frame *)
     (leibnizO R.Local_Ctx -n> leibnizO wlocal_ctx -n> leibnizO instance -n> FR) *
     (* Expression *)
-    (leibnizO (list R.Typ) -n>
-     leibnizO R.Function_Ctx -n>
-     leibnizO R.Local_Ctx -n>
-     leibnizO wlocal_ctx -n>
-     leibnizO instance -n>
-     ER).
+    (leibnizO (list R.Typ) -n> leibnizO R.Function_Ctx -n> leibnizO R.Local_Ctx -n>
+       leibnizO wlocal_ctx -n> leibnizO instance -n> ER).
 
-  Canonical Structure relationsO : ofe := Ofe relations (@prod_ofe_mixin (prodO _ _) _).
+  Definition relations_value_phys (rs : relations) : leibnizO R.Typ -n> WsR :=
+    rs.1.1.
 
-  Program Definition relations_value_phys : relationsO -n> leibnizO R.Typ -n> WsR :=
-    λne rs, rs.1.1.
+  Definition relations_frame (rs : relations) :
+    leibnizO R.Local_Ctx -n> leibnizO wlocal_ctx -n> leibnizO instance -n> FR :=
+    rs.1.2.
 
-  Program Definition relations_frame :
-    relationsO -n> leibnizO R.Local_Ctx -n> leibnizO wlocal_ctx -n> leibnizO instance -n> FR :=
-    λne rs, rs.1.2.
+  Definition relations_expr (rs : relations) :
+    leibnizO (list R.Typ) -n> leibnizO R.Function_Ctx -n> leibnizO R.Local_Ctx -n>
+      leibnizO wlocal_ctx -n> leibnizO instance -n> ER :=
+    rs.2.
 
-  Definition relations_expr :
-    relationsO -n>
-    leibnizO (list R.Typ) -n>
-    leibnizO R.Function_Ctx -n>
-    leibnizO R.Local_Ctx -n>
-    leibnizO wlocal_ctx -n>
-    leibnizO instance -n>
-    ER :=
-    λne rs, snd rs.
+  Definition interp_heap_value_mm_variant (rs : relations) (τs : list R.Typ) : HVmmR :=
+    λne bs,
+      (∃ bs_tag bs_data,
+       ⌜bs = bs_tag ++ bs_data⌝ ∗
+       ∃ tag tag_i32 τ,
+       ⌜wasm_deserialise bs_tag T_i32 = VAL_int32 tag_i32⌝ ∗
+       ⌜nat_repr tag tag_i32⌝ ∗
+       ⌜nth_error τs tag = Some τ⌝ ∗
+       relations_value_phys rs τ (deserialize_values bs_data τ))%I.
 
-  Program Definition interp_heap_value_mm_variant : relationsO -n> leibnizO (list R.Typ) -n> HVmmR :=
-    λne rs τs bs, (
-      ∃ bs_tag bs_data,
-      ⌜bs = bs_tag ++ bs_data⌝ ∗
-      ∃ tag tag_i32 τ,
-      ⌜wasm_deserialise bs_tag T_i32 = VAL_int32 tag_i32⌝ ∗
-      ⌜nat_repr tag tag_i32⌝ ∗
-      ⌜τs !! tag = Some τ⌝ ∗
-      relations_value_phys rs τ (deserialize_values bs_data τ)
-    )%I.
+  Definition interp_heap_value_mm_struct (rs : relations) (fs : list (R.Typ * R.Size)) : HVmmR :=
+    λne bs,
+      (∃ bss,
+       ⌜bs = flatten bss⌝ ∗
+       [∗ list] '(τ, sz); bs' ∈ fs; bss,
+       ⌜length bs' = (4 * R.interp_size (const 0) sz)%nat⌝ ∗
+       relations_value_phys rs τ (deserialize_values bs' τ))%I.
 
-  Program Definition interp_heap_value_mm_struct :
-    relationsO -n> leibnizO (list (R.Typ * R.Size)) -n> HVmmR :=
-    λne rs fs bs, (
-      ∃ bss,
-      ⌜bs = flatten bss⌝ ∗
-      [∗ list] '(τ, sz); bs' ∈ fs; bss,
-      ⌜length bs' = (4 * R.interp_size (const 0) sz)%nat⌝ ∗
-      relations_value_phys rs τ (deserialize_values bs' τ)
-    )%I.
-  Final Obligation.
-    solve_proper_prepare.
-    solve_iprop_ne.
-    apply big_sepL2_ne; intros.
-    destruct y1.
-    solve_iprop_ne.
-    do 4 Morphisms.f_equiv.
-    apply H.
-  Qed.
+  Definition interp_heap_value_mm_array (rs : relations) (τ : R.Typ) : HVmmR :=
+    λne bs,
+      (∃ bs_len bs_elems,
+       ⌜bs = bs_len ++ flatten bs_elems⌝ ∗
+       ∃ len len_i32,
+       ⌜wasm_deserialise bs_len T_i32 = VAL_int32 len_i32⌝ ∗
+       ⌜nat_repr len len_i32⌝ ∗
+       ⌜len = length bs_elems⌝ ∗
+       [∗ list] bs_elem ∈ bs_elems,
+       relations_value_phys rs τ (deserialize_values bs_elem τ))%I.
 
-  Program Definition interp_heap_value_mm_array : relationsO -n> leibnizO R.Typ -n> HVmmR :=
-    λne rs τ bs, (
-      ∃ bs_len bs_elems,
-      ⌜bs = bs_len ++ flatten bs_elems⌝ ∗
-      ∃ len len_i32,
-      ⌜wasm_deserialise bs_len T_i32 = VAL_int32 len_i32⌝ ∗
-      ⌜nat_repr len len_i32⌝ ∗
-      ⌜len = length bs_elems⌝ ∗
-      [∗ list] bs_elem ∈ bs_elems,
-      relations_value_phys rs τ (deserialize_values bs_elem τ)
-    )%I.
+  Definition interp_heap_value_mm_ex (rs : relations) :
+    leibnizO R.Size -n> leibnizO R.Qual -n> leibnizO R.Typ -n> HVmmR :=
+    λne sz q τ bs, False%I.
 
-  Definition interp_heap_value_mm_ex :
-    relationsO -n> leibnizO R.Size -n> leibnizO R.Qual -n> leibnizO R.Typ -n> HVmmR :=
-    λne rs sz q τ bs, False%I.
-
-  Program Definition interp_heap_value_mm (rs : relations) : leibnizO R.HeapType -n> HVmmR :=
-    λne Ψ,
+  Definition interp_heap_value_mm (rs : relations) (Ψ : R.HeapType) : HVmmR :=
     match Ψ with
     | R.VariantType τs => interp_heap_value_mm_variant rs τs
     | R.StructType fs => interp_heap_value_mm_struct rs fs
@@ -130,87 +108,81 @@ Section Relations.
     | R.Ex sz q τ => interp_heap_value_mm_ex rs sz q τ
     end.
 
-  Definition interp_closure (rs : relations) : leibnizO R.FunType -n> ClR :=
-    λne τf cl,
-    let '(R.FunT _ (R.Arrow τ1 τ2)) := τf in
-    match cl with
-    | FC_func_native inst (Tf ts1 ts2) ts_local es => False%I
-    | FC_func_host _ _ => False%I
-    end.
+  Definition interp_closure (rs : relations) (τf : R.FunType) : ClR :=
+    λne cl,
+      let '(R.FunT _ (R.Arrow τ1 τ2)) := τf in
+      match cl with
+      | FC_func_native inst (Tf ts1 ts2) ts_local es => False%I
+      | FC_func_host _ _ => False%I
+      end.
 
-  Program Definition interp_value_phys_coderef (rs : relations) : leibnizO R.FunType -n> WsR :=
-    λne tf ws, (
-      ∃ n,
-      ⌜ws = [VAL_int32 n]⌝ ∗
-      ∃ cl,
-      ▷ interp_closure rs tf cl ∗
-      let n' := Z.to_N (Wasm_int.Int32.unsigned n) in
-      na_inv logrel_nais (ns_func n') (n' ↦[wf] cl)
-    )%I.
+  Definition interp_value_phys_coderef (rs : relations) (tf : R.FunType) : WsR :=
+    λne ws,
+      (∃ n,
+       ⌜ws = [VAL_int32 n]⌝ ∗
+       ∃ cl,
+       ▷ interp_closure rs tf cl ∗
+       let n' := Z.to_N (Wasm_int.Int32.unsigned n) in
+       na_inv logrel_nais (ns_func n') (n' ↦[wf] cl))%I.
 
-  Definition interp_value_phys_exloc (rs : relations) : leibnizO R.Typ -n> WsR :=
-    λne τ ws, (
-      ∃ ℓ c, ▷ relations_value_phys rs (subst_ext (ext R.SLoc (R.LocP ℓ c) id) τ) ws
-    )%I.
+  Definition interp_value_phys_exloc (rs : relations) (τ : R.Typ) : WsR :=
+    λne ws,
+      (∃ ℓ c, ▷ relations_value_phys rs (subst_ext (ext R.SLoc (R.LocP ℓ c) id) τ) ws)%I.
 
-  Program Definition interp_value_phys_ref_mm (rs : relations) (p : R.Ptr) (ψ : R.HeapType) : WsR :=
-    λne ws, (
-      ∃ bs l32,
-      ⌜ws = [VAL_int32 l32]⌝ ∗
-      ⌜ptr_repr (R.LocP p R.LinMem) l32⌝ ∗
-      N.of_nat sr.(sr_mem_mm) ↦[wms][p] bs ∗
-      interp_heap_value_mm rs ψ bs
-    )%I.
+  Definition interp_value_phys_ref_mm (rs : relations) (p : R.Ptr) (Ψ : R.HeapType) : WsR :=
+    λne ws,
+      (∃ bs l32,
+       ⌜ws = [VAL_int32 l32]⌝ ∗
+       ⌜ptr_repr (R.LocP p R.LinMem) l32⌝ ∗
+       N.of_nat sr.(sr_mem_mm) ↦[wms][p] bs ∗
+       interp_heap_value_mm rs Ψ bs)%I.
 
-  Program Definition interp_values_phys (rs : relations) : leibnizO (list R.Typ) -n> WsR :=
-    λne τs ws, (
-      ∃ wss, ⌜ws = flatten wss⌝ ∗ [∗ list] τ; ws' ∈ τs; wss, relations_value_phys rs τ ws'
-    )%I.
+  Definition interp_values_phys (rs : relations) (τs : list R.Typ) : WsR :=
+    λne ws,
+      (∃ wss,
+       ⌜ws = (flatten wss)⌝ ∗
+       [∗ list] τ; ws' ∈ τs; wss, relations_value_phys rs τ ws')%I.
 
-  Program Definition interp_value_phys_0 (rs : relations) : leibnizO R.Typ -n> WsR :=
+  Definition interp_value_phys_0 (rs : relations) : leibnizO R.Typ -n> WsR :=
     λne τ ws,
-    match τ with
-    | R.Num (R.Int _ R.i32) => ∃ n, ⌜ws = [VAL_int32 n]⌝
-    | R.Num (R.Int _ R.i64) => ∃ n, ⌜ws = [VAL_int64 n]⌝
-    | R.Num (R.Float R.f32) => ∃ n, ⌜ws = [VAL_float32 n]⌝
-    | R.Num (R.Float R.f64) => ∃ n, ⌜ws = [VAL_float64 n]⌝
-    | R.TVar _ => False
-    | R.Unit => ∃ n, ⌜ws = [VAL_int32 n]⌝
-    | R.ProdT τs => interp_values_phys rs τs ws
-    | R.CoderefT tf => interp_value_phys_coderef rs tf ws
-    | R.Rec _ _ => False
-    | R.PtrT _ => False
-    | R.ExLoc _ τ => interp_value_phys_exloc rs τ ws
-    | R.OwnR _ => ⌜nilp ws⌝
-    | R.CapT _ _ _ => ⌜nilp ws⌝
-    | R.RefT _ (R.LocP p R.LinMem) ψ => interp_value_phys_ref_mm rs p ψ ws
-    | R.RefT _ (R.LocP p R.GCMem) ψ => False
-    | R.RefT _ (R.LocV _) _ => False
-    end%I.
+      match τ with
+      | R.Num (R.Int _ R.i32) => ∃ n, ⌜ws = [VAL_int32 n]⌝
+      | R.Num (R.Int _ R.i64) => ∃ n, ⌜ws = [VAL_int64 n]⌝
+      | R.Num (R.Float R.f32) => ∃ n, ⌜ws = [VAL_float32 n]⌝
+      | R.Num (R.Float R.f64) => ∃ n, ⌜ws = [VAL_float64 n]⌝
+      | R.TVar _ => False
+      | R.Unit => ∃ n, ⌜ws = [VAL_int32 n]⌝
+      | R.ProdT τs => interp_values_phys rs τs ws
+      | R.CoderefT tf => interp_value_phys_coderef rs tf ws
+      | R.Rec _ _ => False
+      | R.PtrT _ => False
+      | R.ExLoc _ τ => interp_value_phys_exloc rs τ ws
+      | R.OwnR _ => ⌜nilp ws⌝
+      | R.CapT _ _ _ => ⌜nilp ws⌝
+      | R.RefT _ (R.LocP p R.LinMem) ψ => interp_value_phys_ref_mm rs p ψ ws
+      | R.RefT _ (R.LocP p R.GCMem) ψ => False
+      | R.RefT _ (R.LocV _) _ => False
+      end%I.
 
   Definition interp_frame_0 (rs : relations) :
     leibnizO R.Local_Ctx -n> leibnizO wlocal_ctx -n> leibnizO instance -n> FR :=
-    λne L WL i f, (
-      ↪[frame] f ∗
-      ∃ ws_l ws_wl : list value,
-      ⌜f = Build_frame (ws_l ++ ws_wl) i⌝ ∗
-      (* TODO: not right, throws out sizes with (map fst L) *)
-      ▷ interp_values_phys rs (map fst L) ws_l ∗
-      iris_logrel.interp_val WL (immV ws_wl)
-    )%I.
+    λne L WL i f,
+      (↪[frame] f ∗
+       ∃ ws_l ws_wl,
+       ⌜f = Build_frame (ws_l ++ ws_wl) i⌝ ∗
+       (* TODO: not right, throws out sizes with (map fst L) *)
+       ▷ interp_values_phys rs (map fst L) ws_l ∗
+       iris_logrel.interp_val WL (immV ws_wl))%I.
 
-  Program Definition interp_expr_0 (rs : relations) :
-    leibnizO (list R.Typ) -n>
-    leibnizO R.Function_Ctx -n>
-    leibnizO R.Local_Ctx -n>
-    leibnizO wlocal_ctx -n>
-    leibnizO instance -n>
-    ER :=
-    λne τs C L WL i '(lh, e), (
-      WP e {{ v, ∃ ws, ⌜v = immV ws⌝ ∗
-                       interp_values_phys rs τs ws ∗
-                       ∃ f, relations_frame rs L WL i f }}
-    )%I.
+  Definition interp_expr_0 (rs : relations) :
+    leibnizO (list R.Typ) -n> leibnizO R.Function_Ctx -n> leibnizO R.Local_Ctx -n>
+      leibnizO wlocal_ctx -n> leibnizO instance -n> ER :=
+    λne τs C L WL i lh_es,
+      (let '(lh, es) := lh_es in
+       WP es {{ v, ∃ ws,
+                ⌜v = immV ws⌝ ∗
+                interp_values_phys rs τs ws ∗
+                ∃ f, relations_frame rs L WL i f }})%I.
 
   Definition rels_0 (rs : relations) : relations :=
     (interp_value_phys_0 rs, interp_frame_0 rs, interp_expr_0 rs).
@@ -227,8 +199,8 @@ Section Relations.
   Lemma rels_eq : rels ≡ rels_0 rels.
   Proof. apply fixpoint_unfold. Qed.
 
-  Lemma interp_value_phys_eq τs vs :
-    interp_value_phys τs vs ⊣⊢ interp_value_phys_0 rels τs vs.
+  Lemma interp_value_phys_eq τ vs :
+    interp_value_phys τ vs ⊣⊢ interp_value_phys_0 rels τ vs.
   Proof.
     do 2 f_equiv.
     transitivity (rels_0 rels).1.1.
